Start modeling kinds

src/Dafny/jrnl.i.dfy
@@ -1,3 +1,26 @@
-type Addr = (int, int)
+include "pow.dfy"
+
+datatype Addr = Addr(blkno: nat, off: nat)
 type byte = bv8
 type Object = array<byte>
+type Kind = k:int | 0 <= k <= 15
+function kindSize(k: Kind): int {
+    pow(2,k)
+}
+
+lemma kindSize_bounds(k: Kind)
+ensures kindSize(k) <= 4096*8 {
+    pow_increasing(2, k, 15);
+    assert pow(2,15) == 4096*8;
+}
+
+class Jrnl {
+    ghost var data: map<Addr, Object>;
+    ghost var kinds: map<nat, Kind>;
+
+    predicate Valid() reads this {
+        forall a :: a in data ==>
+        && a.blkno in kinds
+        && data[a].Length == kindSize(kinds[a.blkno])
+    }
+}
