src/Dafny/pow.dfy
@@ -1,0 +1,31 @@
+function pow(x:int, k:nat): int decreases k {
+    if k == 0 then 1 else x * pow(x,k-1)
+}
+lemma {:induction k1} pow_plus(x: int, k1: nat, k2: nat)
+requires 1 <= x
+ensures pow(x, k1) * pow(x, k2) == pow(x, k1+k2)
+{
+}
+
+lemma {:induction k} pow_nonneg(x: int, k: nat)
+requires 1 <= x
+ensures 0 <= pow(x, k)
+{
+}
+
+lemma mul_increasing(x1: nat, x2: nat)
+ensures x1 <= x1 * x2
+{
+    // TODO: wat why is this not provable
+    assume false;
+}
+
+lemma {:induction k1} pow_increasing(x: int, k1: nat, k2: nat)
+requires 1 <= x
+ensures pow(x, k1) <= pow(x, k1+k2)
+{
+    pow_nonneg(x, k1);
+    pow_nonneg(x, k2);
+    pow_plus(x, k1, k2);
+    mul_increasing(pow(x,k1), pow(x,k2));
+}
